dinic all proofs finished

Dinic/Compute_Blocking_Residual.thy
@@ -1,6 +1,6 @@
-theory Compute_Blocking_Residual
+theory Compute_Blocking_Residual                 
   imports DFS_Collect_Backtrack_Example Compute_Blocking_Simple "HOL-Library.Product_Lexorder"
-    Graph_Algorithms_Dev.BFS_Example
+    Graph_Algorithms_Dev.BFS_Example Graph_Algorithms_Dev.RBT_Map_Extension
 begin
 
 lemma same_graph_consts: "G.graph_inv = dfs.Graph.graph_inv"
@@ -9,7 +9,7 @@ lemma same_graph_consts: "G.graph_inv = dfs.Graph.graph_inv"
   "DFS_Collect_Backtrack_Example.neighbourhood = 
                           dfs.Graph.neighbourhood"
   "G.graph_inv = dfs.Graph.graph_inv"
-      by (auto simp add: adj_inv_def RBT_Set.empty_def
+  by (auto simp add: adj_inv_def RBT_Set.empty_def
       BFS_Example.neighbourhood_def DFS_Collect_Backtrack_Example.neighbourhood_def)
 
 global_interpretation blocking_simple: blocking_simple where insert = vset_insert and
@@ -41,7 +41,7 @@ definition "find_path F s t =
     else let final_state = dfs_del_dead_impl F t ( dfs_backtrack_initial_state s)
          in  (case return final_state of NotReachable \<Rightarrow> None |
                                          Reachable    \<Rightarrow> 
-              Some (rev (stack final_state), backtrack final_state)))"
+              Some (rev (stack final_state), backtrack final_state)))" for F
 
 value "find_path G 0 10"
 value "find_path G 0 6"
@@ -54,16 +54,18 @@ value "inorder (flow (blocking_simple_loop 0 10 find_path (\<lambda> e. 4) (bloc
 hide_const G edges
 
 lemma find_path_correct:
+  fixes F
   assumes "dfs.Graph.graph_inv F" "dfs.Graph.finite_graph F" "dfs.Graph.finite_vsets F" "s \<noteq> t"
   shows "\<exists>p. vwalk_bet (dfs.Graph.digraph_abs F) s p t \<Longrightarrow>
        \<exists>p del. vwalk_bet (dfs.Graph.digraph_abs F) s p t \<and> find_path F s t = Some (p, del)"
     (is "?asm1 \<Longrightarrow> ?thesis1")
-    "find_path F s t = Some (p, dlt) \<Longrightarrow>
+    and "find_path F s t = Some (p, dlt) \<Longrightarrow>
        acyc (dfs.Graph.digraph_abs F) \<Longrightarrow>
        vwalk_bet (dfs.Graph.digraph_abs F) s p t \<and>
        distinct p \<and>
        (\<forall>e\<in>set dlt. \<nexists>p. e \<in> set (edges_of_vwalk p) \<and> vwalk_bet (dfs.Graph.digraph_abs F) s p t)"
     (is "?asm2 \<Longrightarrow> ?asm3 \<Longrightarrow> ?thesis2")
+
 proof(all \<open>cases "DFS_Collect_Backtrack_Example.neighbourhood F s = vset_empty"\<close>)
   show  "?asm1 \<Longrightarrow> ?thesis1" if asy: "DFS_Collect_Backtrack_Example.neighbourhood F s = vset_empty"
     using assms(4) dfs.Graph.vset.set.set_empty vwalk_then_edge[of "dfs.Graph.digraph_abs F" s _  t] 
@@ -159,7 +161,7 @@ fixes s t ::'v
 begin
 
 definition "pos_es = filter (\<lambda> e. rcap \<f> e > 0) (map F es @ map B es)"
-
+  (*Turn later into join/projection/collapsing functions.*)
 definition "realising_edges_general list =
            (foldr (\<lambda> e found_edges. let ee = to_vertex_pair e in
                      (case realising_edges_lookup found_edges ee of 
@@ -171,13 +173,12 @@ definition "realising_edges = realising_edges_general pos_es"
 
 definition "E_simple = foldr (\<lambda> e acc. add_edge acc (prod.fst e) (prod.snd e))
                           (map to_vertex_pair pos_es) empty"
-
-definition "level_simple = parents (bfs_impl E_simple (bfs_initial_state 
-                          (vset_insert s Pair_Graph_RBT.vset_empty)))"
-
 definition "u_simple e = sum_list (map (\<lambda> e. real_of_ereal (rcap \<f> e)) 
                        (case realising_edges_lookup realising_edges e of None \<Rightarrow> []| 
                         Some ees \<Rightarrow> ees))"
+
+definition "level_simple = parents (bfs_impl E_simple (bfs_initial_state 
+                          (vset_insert s Pair_Graph_RBT.vset_empty)))"
 
 definition "blocking_flow_simple = 
       (if neighbourhood E_simple s = vset_empty 
@@ -186,10 +187,27 @@ definition "blocking_flow_simple =
                  (blocking_simple_initial level_simple))
             in if f = empty then None
             else Some f)"
-
+  (*later, use a split function.*)
 definition "residual_add_flow f e \<gamma> = 
 residual_flow_update e ((abstract_real_map (residual_flow_lookup f) e) + \<gamma>) f"
 
+(*later, use a split function.*)
+
+definition "split_flow_single e fl acc= 
+prod.fst (foldl (\<lambda> (resf, f) ee . 
+       let \<gamma> = min (real_of_ereal (rcap \<f> ee)) f
+       in (residual_add_flow resf ee \<gamma>, f -\<gamma>))
+        (acc, fl) (the (realising_edges_lookup realising_edges e)))"
+
+definition "find_blocking_flow =
+    (case blocking_flow_simple 
+     of None \<Rightarrow> None |
+        Some flw \<Rightarrow>
+     Some (
+       rbt_map_fold flw (\<lambda> e fl acc. split_flow_single e fl acc) 
+         residual_flow_empty
+      ))"
+  (*
 definition "residual_blocking_flow =
     (case blocking_flow_simple 
      of None \<Rightarrow> None |
@@ -209,8 +227,17 @@ definition "residual_blocking_flow =
           )
          (map to_vertex_pair pos_es)
          residual_flow_empty
-      ))"
-
+      ))"*)
+lemmas [code] =pos_es_def
+  realising_edges_general_def
+  realising_edges_def
+  E_simple_def
+  u_simple_def
+  level_simple_def
+  blocking_flow_simple_def
+  residual_add_flow_def
+  find_blocking_flow_def
+  split_flow_single_def
 
 end
 
@@ -234,13 +261,13 @@ lemma pos_es_props: "set pos_es = {e | e. e \<in> \<EE> \<and> rcap \<f> e > 0}"
   "distinct pos_es"
   by (auto intro!: distinct_filter inj_onI 
       simp add: pos_es_def \<EE>_def  distinct_map es_props)
-
+    (*Use for projection*)
 lemma realising_edges_invar_pres: "realising_edges_invar (realising_edges_general list)"
   unfolding realising_edges_general_def
   by(auto intro: foldr_invar 
       simp add: Map_realising.invar_empty Map_realising.invar_update realising_edges_general_def 
       split: option.split)
-
+    (*Use for projection*)
 lemma realising_edges_general_result_None_and_Some:
   assumes "(case realising_edges_lookup (realising_edges_general list) (u, v) 
             of Some ds \<Rightarrow> ds 
@@ -260,7 +287,7 @@ next
         simp add: Map_realising.map_update realising_edges_general_def Cons(2)[symmetric] 
         split: option.split)
 qed
-
+  (*Use for projection*)
 lemma realising_edges_general_result_distinct:
   assumes "distinct list"
     "(case realising_edges_lookup (realising_edges_general list) (u, v) 
@@ -289,24 +316,24 @@ next
         Map_realising.map_update[OF  realising_edges_invar_pres , of "to_vertex_pair e" _ list] 
         split: option.split)
 qed
-
+  (*Use for projection*)
 lemma realising_edges_general_result:
   assumes "realising_edges_lookup (realising_edges_general list) (u, v) = Some ds"
   shows "set ds = {e | e. e \<in> set list \<and> to_vertex_pair e = (u, v)}"
   using realising_edges_general_result_None_and_Some[of list u v ds] assms
   by simp
-
+    (*Use for projection*)
 lemma realising_edges_result:
-  "realising_edges_lookup realising_edges (u, v) = Some ds \<Longrightarrow>
-    set ds = {e |e. e \<in> set pos_es \<and> to_vertex_pair e = (u, v)}"
-  "realising_edges_lookup realising_edges (u, v) = Some ds \<Longrightarrow>
+  "realising_edges_lookup realising_edges d = Some ds \<Longrightarrow>
+    set ds = {e |e. e \<in> set pos_es \<and> to_vertex_pair e = d}"
+  "realising_edges_lookup realising_edges d= Some ds \<Longrightarrow>
     distinct ds"
-  "realising_edges_lookup realising_edges (u, v) = None \<Longrightarrow>
-    {e |e. e \<in> set pos_es \<and> to_vertex_pair e = (u, v)} = {}"
-  using realising_edges_general_result_distinct[OF pos_es_props(2) refl, of u v] 
+  "realising_edges_lookup realising_edges d = None \<Longrightarrow>
+    {e |e. e \<in> set pos_es \<and> to_vertex_pair e = d} = {}"
+  using realising_edges_general_result_distinct[OF pos_es_props(2) refl, of "prod.fst d" "prod.snd d"] 
     realising_edges_general_result_None_and_Some[OF refl] 
-  by(force simp add: realising_edges_def realising_edges_general_result)+
-
+  by(all \<open>cases d\<close>)(force simp add: realising_edges_def realising_edges_general_result)+
+    (*Use for projection*)
 lemma E_simple_props: "dfs.Graph.graph_inv E_simple" (is ?goal1)
   "dfs.Graph.finite_graph E_simple" (is ?goal2)
   "dfs.Graph.finite_vsets E_simple" (is ?goal3)
@@ -326,11 +353,21 @@ proof-
     by(induction list)(auto intro: dfs.Graph.finite_graph_add_edge)
   thus ?goal1 ?goal2 ?goal3 ?goal4 by auto
 qed
+lemma distinct_pairs_no_reaising_in_common:
+  "e \<noteq> d \<Longrightarrow>
+  {x. \<exists>uu. Some uu = realising_edges_lookup realising_edges e \<and> x \<in> set uu} \<inter>
+  {x. \<exists>uu. Some uu = realising_edges_lookup realising_edges d \<and> x \<in> set uu} =
+       {}"
+  using realising_edges_result(1)
+  by(cases "realising_edges_lookup realising_edges e",
+      all \<open>cases "realising_edges_lookup realising_edges d"\<close>)
+    auto
 
+(*Use for projection*)
 lemma u_simple_is:
-  "u_simple (u, v) = (\<Sum>e\<in>{e |e. e \<in> set pos_es \<and> to_vertex_pair e = (u, v)}.
+  "u_simple ee = (\<Sum>e\<in>{e |e. e \<in> set pos_es \<and> to_vertex_pair e = ee}.
                           real_of_ereal \<uu>\<^bsub>\<f>\<^esub>e)"
-  using realising_edges_result[of u v]
+  using realising_edges_result[of ee]
   by(auto intro!: comm_monoid_add_class.sum.neutral 
       split: option.split 
       simp add: u_simple_def,
@@ -361,33 +398,6 @@ lemma bfs_axiom: "neighbourhood E_simple s \<noteq>vset_empty \<Longrightarrow>
                                                   E_simple _", 
         simplified dfs.Graph.neighbourhood_abs[OF  E_simple_props(1)]]
       same_graph_consts(1-3))
-    (*
-lemma level_siple_is: "(bfs_impl E_simple (bfs_initial_state 
-                          (vset_insert s Pair_Graph_RBT.vset_empty))) = 
-                       (bfs.BFS E_simple (bfs_initial_state 
-                          (vset_insert s Pair_Graph_RBT.vset_empty)))"
-*)
-    (*
-interpretation blocking_simple_thms: blocking_simple_thms where insert = vset_insert and
- sel = sel and  vset_empty = vset_empty and  diff = vset_diff and
- lookup = lookup and empty = map_empty and delete=delete and isin = isin and t_set=t_set
-and update=update and adjmap_inv = adj_inv and vset_delete= vset_delete
-and vset_inv = vset_inv and union=vset_union and inter=vset_inter 
-and flow_lookup = lookup
-and flow_empty = Leaf
-and flow_update=update
-and flow_delete=delete
-and flow_invar=adj_inv
-and G = E_simple and
-t = t and
-s = s and
-find_path = find_path and
-u = u
-  apply(auto intro!: blocking_simple_thms.intro) 
-  apply (simp add: blocking_simple.flow_map.Map_axioms blocking_simple.intro
-      dfs.Graph.Pair_Graph_Specs_axioms dfs.set_ops.Set2_axioms)
-  apply(auto intro!: blocking_simple_thms_axioms.intro simp add: E_simple_props)
-  apply (simp add: E_simple_props(1))*)
 
 lemma e_leaving_s_in_level_graph:
   "e\<in>\<EE> \<Longrightarrow> 0 < \<uu>\<^bsub>\<f>\<^esub>e \<Longrightarrow> fstv e = s \<Longrightarrow> sndv e \<noteq> s \<Longrightarrow>
@@ -422,10 +432,14 @@ abbreviation "simple_level_graph_abstract ==  (level_graph (dfs.Graph.digraph_ab
 abbreviation "is_blocking_flow_simple == 
 flow_network_spec.is_blocking_flow prod.fst prod.snd id simple_level_graph_abstract u_simple"
 
-lemma "blocking_flow_simple = None \<Longrightarrow> \<nexists> p. vwalk_bet (dfs.Graph.digraph_abs E_simple) s p t" (is "?none \<Longrightarrow> ?nowalk")
-  "blocking_flow_simple = Some f \<Longrightarrow>\<exists> p. vwalk_bet (dfs.Graph.digraph_abs E_simple) s p t" (is "?some \<Longrightarrow> ?walk")
-  "blocking_flow_simple = Some f \<Longrightarrow> is_blocking_flow_simple s t (abstract_real_map (lookup f))" (is "?some \<Longrightarrow> ?blocking_flow")
-  "blocking_flow_simple = Some f \<Longrightarrow>\<exists>e\<in>\<EE>. 0 < \<uu>\<^bsub>\<f>\<^esub>e \<and> fstv e = s \<and> sndv e \<noteq> s" (is "?some \<Longrightarrow>?leaving_e")
+lemma blocking_flow_simple_correct:
+
+"blocking_flow_simple = None \<Longrightarrow> \<nexists> p. vwalk_bet (dfs.Graph.digraph_abs E_simple) s p t" (is "?none \<Longrightarrow> ?nowalk")
+"blocking_flow_simple = Some f \<Longrightarrow>\<exists> p. vwalk_bet (dfs.Graph.digraph_abs E_simple) s p t" (is "?some \<Longrightarrow> ?walk")
+"blocking_flow_simple = Some f \<Longrightarrow> is_blocking_flow_simple s t (abstract_real_map (lookup f))" (is "?some \<Longrightarrow> ?blocking_flow")
+"blocking_flow_simple = Some f \<Longrightarrow>\<exists>e\<in>\<EE>. 0 < \<uu>\<^bsub>\<f>\<^esub>e \<and> fstv e = s \<and> sndv e \<noteq> s" (is "?some \<Longrightarrow>?leaving_e")
+"blocking_flow_simple = Some f \<Longrightarrow> dom (lookup f) \<subseteq> simple_level_graph_abstract"
+"blocking_flow_simple = Some f \<Longrightarrow> adj_inv f"
 proof(all \<open>cases "neighbourhood E_simple s = vset_empty"\<close>)
   show "?none \<Longrightarrow> neighbourhood E_simple s = vset_empty \<Longrightarrow> ?nowalk"
     by (auto simp add: G.source_of_path_neighb_non_empty RBT_Set.empty_def s_neq_t
@@ -433,11 +447,13 @@ proof(all \<open>cases "neighbourhood E_simple s = vset_empty"\<close>)
         DFS_Collect_Backtrack_Example.neighbourhood_def
         blocking_flow_simple_def same_graph_consts(3))
   show "?some \<Longrightarrow> neighbourhood E_simple s = vset_empty \<Longrightarrow> ?walk"
+    "?some \<Longrightarrow> neighbourhood E_simple s = vset_empty \<Longrightarrow> ?blocking_flow"
+    "?some \<Longrightarrow> BFS_Example.neighbourhood E_simple s = vset_empty \<Longrightarrow> \<exists>e\<in>\<EE>. 0 < \<uu>\<^bsub>\<f>\<^esub>e \<and> fstv e = s \<and> sndv e \<noteq> s"
+    "?some \<Longrightarrow> BFS_Example.neighbourhood E_simple s = vset_empty \<Longrightarrow>
+         dom (lookup f) \<subseteq> simple_level_graph_abstract"
+    "?some \<Longrightarrow> BFS_Example.neighbourhood E_simple s = vset_empty \<Longrightarrow>
+         adj_inv f"
     by (auto simp add:  blocking_flow_simple_def )   
-  show "?some \<Longrightarrow> neighbourhood E_simple s = vset_empty \<Longrightarrow> ?blocking_flow"
-    by (auto simp add:  blocking_flow_simple_def )
-  show "?some \<Longrightarrow> BFS_Example.neighbourhood E_simple s = vset_empty \<Longrightarrow> \<exists>e\<in>\<EE>. 0 < \<uu>\<^bsub>\<f>\<^esub>e \<and> fstv e = s \<and> sndv e \<noteq> s"
-    by (auto simp add:  blocking_flow_simple_def )  
   assume assm1: "neighbourhood E_simple s \<noteq> vset_empty"
   note bfs_axiom = bfs_axiom[OF assm1]
   have level_siple_is: "(bfs_impl E_simple (bfs_initial_state 
@@ -582,8 +598,8 @@ proof(all \<open>cases "neighbourhood E_simple s = vset_empty"\<close>)
   note  flow_network_axioms_for_simple_graph = 
     flow_network_axioms_for_simple_graph[OF residual_leaving_s]
   note is_blocking_flow_def=flow_network_spec.is_blocking_flow_def[of
-            prod.fst prod.snd id
-   "(level_graph (dfs.Graph.digraph_abs E_simple) {s} -
+      prod.fst prod.snd id
+      "(level_graph (dfs.Graph.digraph_abs E_simple) {s} -
     {(u, v) |u v. distance (dfs.Graph.digraph_abs E_simple) s u = \<infinity>})" "(\<lambda>x. ereal (u_simple x))"]
   note bfs_level_graph_def=BFS_level_graph[simplified same_graph_consts(2) srcs_are_s 
       distance_set_single_source, symmetric]
@@ -603,8 +619,849 @@ proof(all \<open>cases "neighbourhood E_simple s = vset_empty"\<close>)
         blocking_flow_simple_def  bfs_level_graph_def if_not_P[OF assm1] Let_def,
         subst (asm) if_not_P)
       (auto simp add: if_not_P)
+  show "dom (lookup f) \<subseteq> simple_level_graph_abstract"
+    using same_final_state blocking_simple_correctness(5) assms2(1)
+      flow_non_empt is_blocking_flow_def[of s t]  not_None_eq option.inject
+    by(unfold prnts_def level_siple_is level_simple_def  blocking_simple_initial_def
+        blocking_flow_simple_def  bfs_level_graph_def if_not_P[OF assm1] Let_def,
+        subst (asm) if_not_P)
+      (auto simp add: if_not_P)
+  show "adj_inv f"
+    using same_final_state blocking_simple_correctness(6) assms2(1)
+      flow_non_empt is_blocking_flow_def[of s t]  not_None_eq option.inject
+    by(unfold prnts_def level_siple_is level_simple_def  blocking_simple_initial_def
+        blocking_flow_simple_def  if_not_P[OF assm1] Let_def,
+        subst (asm) if_not_P)
+      (auto simp add: if_not_P)
+qed
+
+lemma vwalk_simple_to_resreach:
+  assumes "vwalk_bet (dfs.Graph.digraph_abs E_simple) s p t"
+  shows "resreach \<f> s t"
+proof-
+  have awalk_found: "awalk (to_vertex_pair ` 
+          {x. (x \<in> F ` \<E> \<or> x \<in> Redge.B ` \<E>) \<and> 0 < \<uu>\<^bsub>\<f>\<^esub>x}) s
+     (edges_of_vwalk p) t"
+    using vwalk_imp_awalk[OF assms]
+    by (unfold E_simple_props(4) pos_es_def set_filter set_map set_append
+        resreach_def  es_props(1) ) auto
+  then obtain pp where pp:"set pp \<subseteq>
+                {x. (x \<in> F ` \<E> \<or> x \<in> Redge.B ` \<E>) \<and> 0 < \<uu>\<^bsub>\<f>\<^esub>x}"
+    "map to_vertex_pair pp = edges_of_vwalk p" 
+    using list_in_image_map[of "edges_of_vwalk p"] 
+    by(force simp add: awalk_def)
+  have "awalk (to_vertex_pair ` \<EE>) s (map to_vertex_pair pp) t"
+    using awalk_found
+    by(auto intro: subset_mono_awalk simp add:  pp(2)[symmetric] \<EE>_def)
+  moreover have "0 < Rcap \<f> (set pp)"
+    using pp(1) 
+    by(auto intro!: Rcap_strictI')
+  moreover have " pp \<noteq> []" 
+    using pp(2) awalk_found s_neq_t by fastforce
+  moreover have "set pp \<subseteq> \<EE>"
+    using pp(1) 
+    by(auto simp add: \<EE>_def)
+  ultimately show ?thesis
+    by(auto intro!: exI[of _ pp] simp add: resreach_def)
+qed
+
+lemma resreach_to_vwalk_simple:
+  assumes "resreach \<f> s t"
+  shows "\<exists> p. vwalk_bet (dfs.Graph.digraph_abs E_simple) s p t"
+proof-
+  obtain p where p: "awalk (to_vertex_pair ` \<EE>) s (map to_vertex_pair p) t"
+    "Rcap \<f> (set p) > 0" "p \<noteq> []" "set p \<subseteq> \<EE>"
+    using assms by(auto simp add: resreach_def)
+  show ?thesis
+    using p(3)  p(4)
+    by(force intro!: exI[of _ "awalk_verts s (map to_vertex_pair p)"]
+        awalk_imp_vwalk subset_mono_awalk'[OF p(1)] imageI 
+        rcap_extr_strict[OF _ p(2)]
+        simp add: \<EE>_def E_simple_props(4) pos_es_def es_props(1))
+qed
+
+lemma residual_add_flow_correct:
+  assumes "residual_flow_invar acc"
+  shows   "residual_flow_invar (residual_add_flow acc e g)"
+          "dom (residual_flow_lookup (residual_add_flow acc e g))
+               = Set.insert e (dom (residual_flow_lookup acc))"
+          "abstract_real_map (residual_flow_lookup (residual_add_flow acc e g)) =
+           (\<lambda> d. if e = d then abstract_real_map (residual_flow_lookup acc) d + g 
+                          else abstract_real_map (residual_flow_lookup acc) d)"
+          "e \<noteq> d \<Longrightarrow> (residual_flow_lookup (residual_add_flow acc e g)) d =
+                     residual_flow_lookup acc d"
+  using assms
+  by(auto intro!: ext 
+        simp add: residual_add_flow_def abstract_real_map_def 
+                  Map_residual_flow.map_update Map_residual_flow.invar_update 
+           split: option.split if_split)
+
+(*TODO MOVE*)
+lemma ereal_of_real_of_ereal_leq: "x \<ge> 0 \<Longrightarrow> ereal (real_of_ereal x) \<le> x"
+  by (simp add: ereal_real)
+
+  (*To be solved by split lemmas/ to be outsourced*)
+
+lemma split_flow_single_correct1:
+  assumes "residual_flow_invar acc" " realising_edges_lookup realising_edges e = Some ds"
+  shows  "residual_flow_invar (split_flow_single e fl acc)"
+    "dom (residual_flow_lookup  (split_flow_single e fl acc)) \<subseteq>
+          dom (residual_flow_lookup acc) \<union> set (the (realising_edges_lookup realising_edges e))"
+    "\<And> d. d \<notin> set ds \<Longrightarrow>
+         residual_flow_lookup 
+               (split_flow_single e fl acc) d = residual_flow_lookup acc d"
+proof-
+  let ?iteration = " (\<lambda>(resf, f) ee.
+             let \<gamma> = min (real_of_ereal \<uu>\<^bsub>\<f>\<^esub>ee) f in (residual_add_flow resf ee \<gamma>, f - \<gamma>))"
+  have resflow_invar_fold:"residual_flow_invar acc \<Longrightarrow> residual_flow_invar
+     (prod.fst (foldl ?iteration (acc, fl) ds))" for ds fl acc
+    using assms(1)
+    by(induction ds arbitrary: acc fl)
+      (auto intro: residual_add_flow_correct(1) split: prod.split)
+  thus "residual_flow_invar (split_flow_single e fl acc)"
+    using assms(1)
+    by(simp add: split_flow_single_def)
+  have no_change_outside_es: 
+       "residual_flow_invar acc \<Longrightarrow> e \<notin> set ds\<Longrightarrow> residual_flow_lookup
+     (prod.fst (foldl ?iteration (acc, fl) ds)) e = 
+       residual_flow_lookup acc e" for ds fl acc e
+    using assms(1)  Map_residual_flow.map_update residual_add_flow_correct(1,4)
+    by (induction ds arbitrary: acc fl)auto
+  thus " d \<notin> set ds \<Longrightarrow>
+         residual_flow_lookup 
+               (split_flow_single e fl acc) d = residual_flow_lookup acc d" for d
+    by (simp add: assms(1,2) split_flow_single_def)
+  have "residual_flow_invar acc \<Longrightarrow> 
+       dom (residual_flow_lookup (prod.fst (foldl ?iteration (acc, fl) ds ))) = 
+        set ds \<union> dom (residual_flow_lookup acc)" for ds
+  proof(induction ds arbitrary: acc fl)
+    case (Cons a ds)
+    show ?case  
+      using residual_add_flow_correct(2) Cons(1)[simplified case_prod_beta Let_def]
+     by (unfold set_simps(2) Un_insert_left 
+                foldl_Cons case_prod_beta )
+          (auto simp add:  Cons.prems residual_add_flow_correct(1))
+  qed auto
+  thus "dom (residual_flow_lookup (split_flow_single e fl acc))
+    \<subseteq> dom (residual_flow_lookup acc) \<union> set (the (realising_edges_lookup realising_edges e))"  
+    using assms(1) by(simp add:  split_flow_single_def)
+qed
+
+lemma split_flow_single_correct2:
+  assumes "residual_flow_invar acc" " realising_edges_lookup realising_edges e = Some ds"
+    "(\<And> d. d \<in> set ds\<Longrightarrow> abstract_real_map (residual_flow_lookup acc) d= 0)"
+    "fl \<le> u_simple e" "fl \<ge> 0"
+  shows  
+    "sum (abstract_real_map (residual_flow_lookup  (split_flow_single e fl acc)))
+           (set ds) = fl"
+    "\<And> d. d \<in> set ds \<Longrightarrow>
+         abstract_real_map (residual_flow_lookup 
+               (split_flow_single e fl acc)) d \<le> rcap \<f> d"
+    "\<And> d. d \<in> set ds \<Longrightarrow>
+         abstract_real_map (residual_flow_lookup 
+               (split_flow_single e fl acc)) d \<ge> 0"
+proof-
+  let ?iteration = " (\<lambda>(resf, f) ee.
+             let \<gamma> = min (real_of_ereal \<uu>\<^bsub>\<f>\<^esub>ee) f in (residual_add_flow resf ee \<gamma>, f - \<gamma>))"
+  have resflow_invar_fold:"residual_flow_invar acc \<Longrightarrow> residual_flow_invar
+     (prod.fst (foldl ?iteration (acc, fl) ds))" for ds fl acc
+    using assms(1)
+    by(induction ds arbitrary: acc fl)
+      (auto intro: residual_add_flow_correct(1) split: prod.split)
+  have no_change_outside_es: 
+       "residual_flow_invar acc \<Longrightarrow> e \<notin> set ds\<Longrightarrow> residual_flow_lookup
+     (prod.fst (foldl ?iteration (acc, fl) ds)) e = 
+       residual_flow_lookup acc e" for ds fl acc e
+    using assms(1)  Map_residual_flow.map_update residual_add_flow_correct(1,4)
+    by (induction ds arbitrary: acc fl)auto
+  note  ds_positive = preorder_class.eq_refl[OF realising_edges_result(1)[OF assms(2),
+                simplified pos_es_props(1)]]
+  show "sum (abstract_real_map (residual_flow_lookup 
+                (split_flow_single e fl acc))) (set ds) = fl"
+    using assms(4)[simplified u_simple_def assms(2), simplified] assms(5)
+          realising_edges_result(2)[OF assms(2)] ds_positive  assms(1,3)
+    unfolding split_flow_single_def assms(2) option.sel
+  proof(induction ds arbitrary: fl acc)
+    case Nil
+    then show ?case by simp
+  next
+    case (Cons a ds)
+    hence distinctds: "distinct ds" by auto
+    have sum_us_pos: "0 \<le> (\<Sum>e\<leftarrow>ds. real_of_ereal \<uu>\<^bsub>\<f>\<^esub>e)"
+      using local.Cons(5) 
+      by(auto intro!: ordered_comm_monoid_add_class.sum_nonneg  real_of_ereal_pos
+            simp add: comm_monoid_add_class.sum.distinct_set_conv_list[OF distinctds, symmetric])
+    have new_fl_less: "fl - min (real_of_ereal \<uu>\<^bsub>\<f>\<^esub>a) fl \<le> (\<Sum>e\<leftarrow>ds. real_of_ereal \<uu>\<^bsub>\<f>\<^esub>e)"
+      using Cons(2) sum_us_pos by auto
+    show ?case 
+      using Cons(4,5,6)  Cons(1)[ OF new_fl_less _ distinctds, simplified Let_def]   
+            residual_add_flow_correct
+            abstract_real_map_cong[of "residual_flow_lookup _ " _ "residual_flow_lookup _",
+                     OF no_change_outside_es[simplified Let_def , of _ a,
+                           OF residual_add_flow_correct(1)[OF Cons(6)]]]
+      by (subst set_simps(2), subst comm_monoid_add_class.sum.insert)
+         (force simp add: Cons.prems(5,6) residual_add_flow_correct(3))+
+  qed
+  fix d
+  assume asm: "d \<in> set ds"
+  show "ereal (abstract_real_map (residual_flow_lookup (split_flow_single e fl acc)) d) \<le> \<uu>\<^bsub>\<f>\<^esub>d"
+    using realising_edges_result(2)[OF assms(2)] ds_positive assms(1,3) asm
+    unfolding split_flow_single_def assms(2) option.sel
+  proof(induction ds arbitrary: acc fl)
+    case Nil
+    then show ?case by auto
+    next
+    case (Cons dd ds)
+    show ?case
+    proof(cases "dd = d")
+      case True
+      show ?thesis 
+       using abstract_real_map_cong[of "residual_flow_lookup _ " _ "residual_flow_lookup _",
+                     OF no_change_outside_es[simplified Let_def , of _ d ds,
+                           OF residual_add_flow_correct(1)[OF Cons(4)]]]
+          True  residual_add_flow_correct(3) Cons(2-6)
+        by(auto intro!: linorder_class.min.coboundedI1 ereal_of_real_of_ereal_leq)
+    next
+      case False
+      show ?thesis 
+        using Cons.prems residual_add_flow_correct(1,3)  False
+        by(auto intro!: Cons(1)[simplified Let_def])
+    qed
+  qed
+  show "(abstract_real_map (residual_flow_lookup (split_flow_single e fl acc)) d) \<ge> 0"
+    using realising_edges_result(2)[OF assms(2)] ds_positive assms(1,3,5) asm
+    unfolding split_flow_single_def assms(2) option.sel
+  proof(induction ds arbitrary: acc fl)
+    case Nil
+    then show ?case by auto
+    next
+    case (Cons dd ds)
+    show ?case
+    proof(cases "dd = d")
+      case True
+      have "0 \<le> real_of_ereal \<uu>\<^bsub>\<f>\<^esub>d"
+        using Cons.prems(2) True real_of_ereal_pos by force 
+      then show ?thesis 
+        using  abstract_real_map_cong[of "residual_flow_lookup _ " _ "residual_flow_lookup _",
+                     OF no_change_outside_es[simplified Let_def , of _ d ds,
+                           OF residual_add_flow_correct(1)[OF Cons(4)]]]
+               True residual_add_flow_correct(3) Cons(2-6)
+        by auto
+    next
+      case False
+      show ?thesis 
+        using Cons.prems residual_add_flow_correct(1,3)  False
+        by(auto intro!: Cons(1)[simplified Let_def])
+    qed
+  qed
+qed
+
+lemma find_blocking_flow_properties:
+  assumes "find_blocking_flow = Some rsfl"
+  shows   "residual_flow_invar rsfl"
+    "dom (residual_flow_lookup rsfl) 
+           \<subseteq> \<Union> {set (the (realising_edges_lookup realising_edges e)) 
+               | e. e \<in> dom (lookup (the blocking_flow_simple) )}"
+    "\<And> e. e \<in> dom (residual_flow_lookup rsfl) \<Longrightarrow>
+            ereal (abstract_real_map (residual_flow_lookup rsfl) e) \<le> rcap \<f> e"
+    "\<And> e. e \<in> dom (residual_flow_lookup rsfl) \<Longrightarrow>
+            abstract_real_map (residual_flow_lookup rsfl) e \<ge> 0"
+    "\<And> e. abstract_real_map (lookup (the blocking_flow_simple) ) e =
+              sum (abstract_real_map (residual_flow_lookup rsfl))
+                  (set (case (realising_edges_lookup realising_edges e) of Some ds \<Rightarrow> ds
+                   | None  \<Rightarrow> []))" 
+proof-
+  have rsfl_is:"rsfl = rbt_map_fold  (the blocking_flow_simple) (\<lambda> e fl acc. split_flow_single e fl acc) 
+         residual_flow_empty"
+    using assms(1)
+    by(cases blocking_flow_simple)(auto simp add: find_blocking_flow_def )
+  obtain bfs where bfs_prop:"blocking_flow_simple = Some bfs" 
+    using assms(1)
+    by(cases blocking_flow_simple)(auto simp add: find_blocking_flow_def )
+  obtain xs where iteration_order: "distinct xs"
+     "set xs = dom (lookup bfs)"
+     "rbt_map_fold bfs split_flow_single residual_flow_empty =
+     foldr (\<lambda>x. split_flow_single x (the (lookup bfs x))) xs residual_flow_empty"
+    using   rbt_map_fold_correct[OF blocking_flow_simple_correct(6)
+             [OF bfs_prop , simplified  adj_inv_def], of split_flow_single residual_flow_empty]
+    by auto
+
+  note simple_flow_in_lg = blocking_flow_simple_correct(5)[OF bfs_prop]
+
+  have in_xs_realising_no_none:"e \<in> set xs \<Longrightarrow>
+           realising_edges_lookup realising_edges e \<noteq> None " for e
+    using order.trans[OF simple_flow_in_lg 
+              order.trans[OF _ level_graph_subset_graph[of 
+             "(dfs.Graph.digraph_abs E_simple)" "{s}"]]]
+         realising_edges_result(3)[of e]
+    by(auto simp add: E_simple_props(4) pos_es_props(1) iteration_order(2))
+  have resflow_invar:"residual_flow_invar
+     (foldr (\<lambda>x. split_flow_single x (the (lookup bfs x))) xs residual_flow_empty)"
+    if "\<And> e. e \<in> set xs \<Longrightarrow>
+           realising_edges_lookup realising_edges e \<noteq> None" for xs
+    using that
+  proof(induction xs)
+    case Nil
+    then show ?case by(auto simp add: Map_residual_flow.invar_empty)
+  next
+    case (Cons a xs)
+    show ?case 
+      using Cons(2)[of a]
+      by(auto intro!: split_flow_single_correct1(1)  Cons(1) Cons(2)[simplified]
+            intro: prod.exhaust[of a]) 
+  qed
+  thus "residual_flow_invar rsfl"
+    using bfs_prop in_xs_realising_no_none iteration_order(3) rsfl_is by auto
+
+  have dom_in:"dom ( residual_flow_lookup
+     (foldr (\<lambda>x. split_flow_single x (the (lookup bfs x))) xs residual_flow_empty))
+     \<subseteq>  \<Union>  {set (the (realising_edges_lookup realising_edges e)) |e.
+          e \<in> set xs}" 
+    if in_xs_realising_no_none: 
+       "\<And> e. e \<in> set xs \<Longrightarrow> realising_edges_lookup realising_edges e \<noteq> None" for xs
+    using in_xs_realising_no_none
+    unfolding iteration_order(2)[symmetric]
+  proof(induction xs)
+    case Nil
+    then show ?case 
+      by (simp add: Map_residual_flow.map_empty)
+  next
+    case (Cons a xs)
+    obtain b where b_obtain:"realising_edges_lookup realising_edges a = Some b"
+      using Cons(2)[of a] by auto
+    show ?case 
+    unfolding foldr_Cons o_apply
+    using resflow_invar[OF Cons(2) ]  Cons(1)[OF Cons(2), simplified]
+    by (intro order.trans[OF split_flow_single_correct1(2), OF _ b_obtain],
+        all \<open>(subst  set_simps(2) image_Collect[symmetric])?\<close>)auto
+qed
+  show dom_subset_descr:"dom (residual_flow_lookup rsfl)
+    \<subseteq> \<Union> {set (the (realising_edges_lookup realising_edges e)) |e.
+          e \<in> dom (lookup (the blocking_flow_simple))}"
+    using dom_in[OF in_xs_realising_no_none, of xs] 
+    by(simp add: bfs_prop iteration_order(2,3) rsfl_is)
+  have "e \<in> dom (residual_flow_lookup rsfl)
+       \<Longrightarrow> ereal (abstract_real_map (residual_flow_lookup rsfl) e) \<le> rcap \<f> e
+           \<and> (abstract_real_map (residual_flow_lookup rsfl) e) \<ge> 0"
+    for e
+    using in_xs_realising_no_none iteration_order(1)
+          equalityD1[OF iteration_order(2)]
+    unfolding rsfl_is bfs_prop option.sel
+    unfolding  iteration_order(3)
+  proof (induction xs)
+    case Nil
+    then show ?case 
+      by (simp add: Map_residual_flow.map_empty)
+  next
+    case (Cons a xs)
+    hence immediately_fom_IH_prems: 
+    "e \<in> set xs \<Longrightarrow> realising_edges_lookup realising_edges e \<noteq> None" 
+    "distinct xs" for e by auto
+    obtain ds where ds_obtain: "realising_edges_lookup realising_edges a = Some ds"
+      using Cons(3)[of a] by auto
+    have d_in_ds_outside_of_old_dom:
+             "d \<notin> \<Union> {set (the (realising_edges_lookup realising_edges e)) |e. e \<in> set xs}"
+      if "d \<in> set ds" for d
+    proof(rule ccontr, goal_cases)
+      case 1
+      then obtain e where e:"e \<in> set xs" "d \<in> set (the (realising_edges_lookup realising_edges e))"
+        by auto
+      then obtain ds' where ds': "realising_edges_lookup realising_edges e = Some ds'"
+        using Cons.prems(2)[of e] by(cases "realising_edges_lookup realising_edges e") auto
+      have "e = a"
+        using realising_edges_result(1)[OF ds'] realising_edges_result(1)[OF ds_obtain]
+              e(2) ds' that by auto
+      thus False
+        using Cons.prems(3) e(1) by auto
+    qed
+    have lookup_less_u_gtr_0_simple:"the (lookup bfs a) \<le> u_simple a" "0 \<le> the (lookup bfs a)"
+    proof-
+      have a_in_dom: "a \<in> dom (lookup bfs)"
+        using Cons.prems(4) by auto
+      show "the (lookup bfs a) \<le> u_simple a" "0 \<le> the (lookup bfs a)"
+        apply(all \<open>rule flow_network_spec.is_blocking_flowE[OF 
+                             blocking_flow_simple_correct(3)[OF  bfs_prop]]\<close>)
+        using set_mp[OF simple_flow_in_lg  a_in_dom]
+        by(auto elim!: flow_network_spec.is_s_t_flowE flow_network_spec.isuflowE 
+             simp add: abstract_real_map_in_dom_the[OF a_in_dom, symmetric])
+    qed    
+    show ?case 
+    proof(cases "e \<in> set ds")
+      case True
+      show ?thesis 
+      using split_flow_single_correct2(2,3)[OF  _ ds_obtain]  lookup_less_u_gtr_0_simple True
+          contra_subsetD[OF dom_in[OF immediately_fom_IH_prems(1), of xs]
+                              d_in_ds_outside_of_old_dom] 
+       by(force intro!: Cons(3) resflow_invar[of xs] abstract_real_map_outside_dom)+
+  next
+    case False
+    note flow_no_change =  split_flow_single_correct1(3)[OF resflow_invar[OF immediately_fom_IH_prems(1)]
+           ds_obtain False, of xs, simplified]
+    note flow_no_change_abstract = abstract_real_map_cong[of "residual_flow_lookup _" e "residual_flow_lookup _", 
+            OF  flow_no_change]
+    show ?thesis
+      using Cons.prems(1) flow_no_change  immediately_fom_IH_prems  Cons.prems(4) 
+      by(auto intro!: conjunct1[OF Cons(1)] conjunct2[OF Cons(1)] simp add: flow_no_change_abstract)
+    qed
+  qed
+  thus "ereal (abstract_real_map (residual_flow_lookup rsfl) e) \<le> \<uu>\<^bsub>\<f>\<^esub>e" 
+       "0 \<le> abstract_real_map (residual_flow_lookup rsfl) e"
+       if "e \<in> dom (residual_flow_lookup rsfl)" for e
+    using that by auto
+  have sum_split:"e \<in> set xs \<Longrightarrow> abstract_real_map (lookup (the blocking_flow_simple)) e =
+         sum (abstract_real_map (residual_flow_lookup rsfl))
+             (set (the (realising_edges_lookup realising_edges e)))" for e
+   using in_xs_realising_no_none iteration_order(1)
+          equalityD1[OF iteration_order(2)]
+    unfolding rsfl_is bfs_prop option.sel  iteration_order(3)
+  proof (induction xs)
+    case Nil
+    then show ?case 
+      by (simp add: Map_residual_flow.map_empty)
+  next
+    case (Cons a xs)
+    hence immediately_fom_IH_prems: 
+    "e \<in> set xs \<Longrightarrow> realising_edges_lookup realising_edges e \<noteq> None" 
+    "distinct xs" for e by auto
+    obtain ds where ds_obtain: "realising_edges_lookup realising_edges a = Some ds"
+      using Cons(3)[of a] by auto
+    have d_in_ds_outside_of_old_dom:
+             "d \<notin> \<Union> {set (the (realising_edges_lookup realising_edges e)) |e. e \<in> set xs}"
+      if "d \<in> set ds" for d
+    proof(rule ccontr, goal_cases)
+      case 1
+      then obtain e where e:"e \<in> set xs" "d \<in> set (the (realising_edges_lookup realising_edges e))"
+        by auto
+      then obtain ds' where ds': "realising_edges_lookup realising_edges e = Some ds'"
+        using Cons.prems(2)[of e] by(cases "realising_edges_lookup realising_edges e") auto
+      have "e = a"
+        using realising_edges_result(1)[OF ds'] realising_edges_result(1)[OF ds_obtain]
+              e(2) ds' that by auto
+      thus False
+        using Cons.prems(3) e(1) by auto
+    qed
+    have lookup_less_u_gtr_0_simple:"the (lookup bfs a) \<le> u_simple a" "0 \<le> the (lookup bfs a)"
+    proof-
+      have a_in_dom: "a \<in> dom (lookup bfs)"
+        using Cons.prems(4) by auto
+      show "the (lookup bfs a) \<le> u_simple a" "0 \<le> the (lookup bfs a)"
+        apply(all \<open>rule flow_network_spec.is_blocking_flowE[OF 
+                             blocking_flow_simple_correct(3)[OF  bfs_prop]]\<close>)
+        using set_mp[OF simple_flow_in_lg  a_in_dom]
+        by(auto elim!: flow_network_spec.is_s_t_flowE flow_network_spec.isuflowE 
+             simp add: abstract_real_map_in_dom_the[OF a_in_dom, symmetric])
+    qed  
+    have the_lookup_abstract:"the (lookup bfs a) = abstract_real_map (lookup bfs) a"
+      using Cons.prems(4) abstract_real_map_in_dom_the by force
+    show ?case 
+    proof(cases "e = a")
+      case True
+      have flow_zero_old: "d \<in> set (the (realising_edges_lookup realising_edges a)) \<Longrightarrow>
+         abstract_real_map
+          (residual_flow_lookup
+            (foldr (\<lambda>x. split_flow_single x (the (lookup bfs x))) xs residual_flow_empty))
+          d = 0" for d
+        using d_in_ds_outside_of_old_dom[of d]
+              dom_in[OF immediately_fom_IH_prems(1), of xs, simplified] 
+        by(auto intro!: abstract_real_map_none simp add: ds_obtain) blast
+      show ?thesis 
+        using flow_zero_old lookup_less_u_gtr_0_simple
+        by(auto intro!: split_flow_single_correct2(1)[symmetric]
+         simp add: True immediately_fom_IH_prems(1) resflow_invar ds_obtain the_lookup_abstract)
+  next
+    case False
+    show ?thesis
+    proof(subst foldr_Cons, subst o_apply, rule trans[OF Cons(1)], goal_cases)
+      case 1
+      then show ?case 
+        using Cons.prems(1) False by auto
+    next
+      case (2 e)
+      then show ?case 
+        using immediately_fom_IH_prems(1) by blast
+    next
+      case 3
+      then show ?case 
+        using immediately_fom_IH_prems(2) by auto
+    next
+      case 4
+      then show ?case
+        using Cons.prems(4) by auto
+    next
+      case 5
+      show ?case 
+      proof(rule sum_cong, goal_cases)
+        case (1 d)
+        hence d_not_in_ds:"d \<notin> set ds" 
+          using  Cons.prems(1) False d_in_ds_outside_of_old_dom[of d] 
+                 ds_obtain immediately_fom_IH_prems(1) realising_edges_result(1) 
+          by auto
+        note flow_no_change =  split_flow_single_correct1(3)[OF resflow_invar[OF immediately_fom_IH_prems(1)]
+           ds_obtain d_not_in_ds, of xs, simplified]
+        then show ?case 
+          by (auto intro!: abstract_real_map_cong)
+      qed
+    qed
+  qed
+qed
+  show "abstract_real_map (lookup (the blocking_flow_simple)) e =
+         sum (abstract_real_map (residual_flow_lookup rsfl))
+          (set (case realising_edges_lookup realising_edges e of None \<Rightarrow> [] | Some ds \<Rightarrow> ds))" for e
+  proof(cases "e \<in> set xs")
+    case True
+    show ?thesis 
+      by (simp add: sum_split True in_xs_realising_no_none option.case_eq_if)
+  next
+    case False
+    hence "abstract_real_map (lookup (the blocking_flow_simple)) e = 0"
+      by(auto intro!: abstract_real_map_outside_dom simp add: bfs_prop domI iteration_order(2))
+    moreover have "realising_edges_lookup realising_edges e = Some ds \<Longrightarrow>
+           sum (abstract_real_map (residual_flow_lookup rsfl)) (set ds) = 0" for ds
+    proof(rule comm_monoid_add_class.sum.neutral
+                        abstract_real_map_outside_dom, rule, 
+         rule abstract_real_map_outside_dom, rule ccontr,
+          goal_cases)
+      case (1 e')
+      then obtain ee where ee:
+        "e' \<in> set (the (realising_edges_lookup realising_edges ee))" "ee \<in> dom (lookup bfs)" 
+        "ee \<in> set xs"
+        using dom_subset_descr by(force simp add: bfs_prop iteration_order(2)) 
+      moreover have "ee = e" 
+        using   in_xs_realising_no_none[of ee] 
+                realising_edges_result(1)[of ee]  "1"(1,2) calculation(1) ee(3)
+                realising_edges_result(1) by auto
+      ultimately show False
+        using False by blast
+    qed
+    ultimately show ?thesis 
+      by(cases "realising_edges_lookup realising_edges e") simp+
+  qed 
+qed
+
+    (*TODO MOVE*)
+lemma sum_split_off: "A \<subseteq> B \<Longrightarrow> finite B \<Longrightarrow> (\<And> x. x \<in> B - A \<Longrightarrow> f x = 0) \<Longrightarrow> sum f A = sum f B" for f A B
+  by (simp add: sum.mono_neutral_cong_right)
+
+lemma if_non_empty_finite_finite: " (A \<noteq> {} \<Longrightarrow> finite A) \<Longrightarrow> finite A" by auto
+
+lemma find_blocking_flow:
+  "find_blocking_flow  = None
+            \<longleftrightarrow> \<not> resreach \<f> s t" (is ?thesis1)
+  "\<And> rf. find_blocking_flow = Some rf \<Longrightarrow> residual_flow_invar rf" 
+  (is "\<And> rf. ?asm1 rf \<Longrightarrow> ?thesis2 rf")
+  "\<And> rf. find_blocking_flow = Some rf \<Longrightarrow>
+         residual_level_blocking_flow  \<f> s t
+                (abstract_real_map (residual_flow_lookup rf))"
+  (is "\<And> rf. ?asm1 rf \<Longrightarrow> ?thesis3 rf")
+  "\<And> rf. find_blocking_flow = Some rf \<Longrightarrow>
+          dom (residual_flow_lookup rf) 
+          \<subseteq> residual_level_graph \<f> s"
+  (is "\<And> rf. ?asm1 rf \<Longrightarrow> ?thesis4 rf")
+proof-
+  show ?thesis1
+    using blocking_flow_simple_correct(1,2)  resreach_to_vwalk_simple  vwalk_simple_to_resreach
+    by (auto split: option.split simp add: find_blocking_flow_def)
+  fix rf
+  assume asm: "find_blocking_flow = Some rf"
+  then obtain rfs where asm':"blocking_flow_simple = Some rfs"
+    by(auto simp add: find_blocking_flow_def 
+        intro: option.exhaust[of blocking_flow_simple])
+  show "residual_flow_invar rf"
+    by (simp add: asm find_blocking_flow_properties(1))
+  have dom_goal:"dom (residual_flow_lookup rf) \<subseteq> residual_level_graph \<f> s 
+                - {e | e. multigraph_spec.multigraph_distance 
+                  {e | e. e \<in> \<EE> \<and> rcap \<f> e > 0} to_vertex_pair s (fstv e) = \<infinity>}"
+  proof(rule order.trans[OF find_blocking_flow_properties(2)[OF asm]],
+      rule Union_least, goal_cases)
+    case (1 X)
+    then obtain e where X_props:"X = set (the (realising_edges_lookup realising_edges e))"
+      "e \<in> dom (lookup (the blocking_flow_simple))" by auto
+    hence e_in_lg: "e \<in> level_graph (dfs.Graph.digraph_abs E_simple) {s} -
+   {(u, v) |u v. distance (dfs.Graph.digraph_abs E_simple) s u = \<infinity>}"
+      using blocking_flow_simple_correct(5) asm' by auto
+    then obtain ds where ds_prop: "realising_edges_lookup realising_edges e = Some ds"
+      using realising_edges_result(3)[of e]
+        level_graph_subset_graph[of "(dfs.Graph.digraph_abs E_simple)" "{s}"]
+      by(fastforce simp add: E_simple_props(4) pos_es_props(1) )
+
+    show ?case
+      using e_in_lg 
+      by(auto simp add: X_props(1) ds_prop  realising_edges_result(1)[OF ds_prop]  
+          residual_level_graph_def multigraph_spec.multi_level_graph_def E_simple_props(4)
+          pos_es_props(1)  multigraph_spec.multigraph_distance_set_def level_graph_def 
+          to_vertex_pair_fst_snd multigraph_spec.multigraph_distance_def)
+  qed
+  thus "dom (residual_flow_lookup rf) \<subseteq> residual_level_graph \<f> s" by auto
+  have valid_s_t_flow: "flow_network_spec.is_s_t_flow fstv sndv to_vertex_pair (residual_level_graph \<f> s) (rcap \<f>)
+     (abstract_real_map (residual_flow_lookup rf)) s t"
+  proof-
+    have uflow:"flow_network_spec.isuflow (residual_level_graph \<f> s) (rcap \<f>)
+     (abstract_real_map (residual_flow_lookup rf))"
+    proof(rule flow_network_spec.isuflowI, goal_cases)
+      case (1 e)
+      then show ?case 
+        apply(cases "e \<in> dom (residual_flow_lookup rf)")
+        subgoal
+          by(auto intro: find_blocking_flow_properties(3)[OF asm])
+        using residual_level_graph_in_E_pos[of \<f> s]
+        by(auto simp add: abstract_real_map_none less_eq_ereal_def zero_ereal_def domIff) 
+    next
+      case (2 e)
+      then show ?case
+        apply(cases "e \<in> dom (residual_flow_lookup rf)")
+        subgoal
+          by(auto intro: find_blocking_flow_properties(4)[OF asm])
+        using residual_level_graph_in_E_pos[of \<f> s]
+        by(auto simp add: abstract_real_map_none less_eq_ereal_def zero_ereal_def domIff) 
+    qed
+    have same_excess: "flow_network_spec.ex fstv sndv (residual_level_graph \<f> s)
+          (abstract_real_map (residual_flow_lookup rf)) x = 
+           flow_network_spec.ex prod.fst prod.snd
+            (level_graph (dfs.Graph.digraph_abs E_simple) {s} -
+            {(u, v) |u v. distance (dfs.Graph.digraph_abs E_simple) s u = \<infinity>})
+            (abstract_real_map (lookup rfs)) x" for x
+    proof-
+      have helper_minus: "e \<in> multigraph_spec.delta_minus (residual_level_graph \<f> s) sndv x \<Longrightarrow>
+    abstract_real_map (residual_flow_lookup rf) e \<noteq> 0 \<Longrightarrow>
+       \<exists>ee\<in>multigraph_spec.delta_minus
+         (level_graph (dfs.Graph.digraph_abs E_simple) {s} -
+          {uu. \<exists>u. (\<exists>v. uu = (u, v)) \<and> distance (dfs.Graph.digraph_abs E_simple) s u = \<infinity>})
+         prod.snd x.
+       \<exists>uu. Some uu = realising_edges_lookup realising_edges ee \<and> e \<in> set uu" for e 
+        using dom_goal realising_edges_result(1,3)[of "make_pair_residual e"]
+        by(auto dest: option.exhaust[of "realising_edges_lookup realising_edges
+                                       (make_pair_residual e)"]
+              elim!: abstract_real_map_not_zeroE[of "residual_flow_lookup rf" ]
+              intro!: exI[of _ "fstv e"]
+              simp add: to_vertex_pair_fst_snd multigraph_spec.delta_minus_def residual_level_graph_def
+              multigraph_spec.multi_level_graph_def multigraph_spec.multigraph_distance_set_def
+              level_graph_def E_simple_props(4) pos_es_props(1)  distance_set_def 
+              multigraph_spec.multigraph_distance_def)
+      have helper_plus: "e \<in> multigraph_spec.delta_plus (residual_level_graph \<f> s) fstv x \<Longrightarrow>
+         abstract_real_map (residual_flow_lookup rf) e \<noteq> 0 \<Longrightarrow>
+         \<exists>x\<in>multigraph_spec.delta_plus
+              (level_graph (dfs.Graph.digraph_abs E_simple) {s} -
+               {uu. \<exists>u. (\<exists>v. uu = (u, v)) \<and> distance (dfs.Graph.digraph_abs E_simple) s u = \<infinity>})
+              prod.fst x.
+            \<exists>uu. Some uu = realising_edges_lookup realising_edges x \<and> e \<in> set uu" for e
+        using dom_goal realising_edges_result(1,3)[of "make_pair_residual e"]
+        by(auto dest: option.exhaust[of "realising_edges_lookup realising_edges
+                                       (make_pair_residual e)"]
+              elim!: abstract_real_map_not_zeroE[of "residual_flow_lookup rf" ]
+              intro!: exI[of _ "sndv e"]
+              simp add: to_vertex_pair_fst_snd multigraph_spec.delta_plus_def residual_level_graph_def
+              multigraph_spec.multi_level_graph_def multigraph_spec.multigraph_distance_set_def
+              level_graph_def E_simple_props(4) pos_es_props(1)  distance_set_def 
+              multigraph_spec.multigraph_distance_def)
+
+      have same_big_sum_minus: "sum (abstract_real_map (residual_flow_lookup rf))
+          (multigraph_spec.delta_minus (residual_level_graph \<f> s) sndv x) =
+          sum (abstract_real_map (residual_flow_lookup rf))
+         (\<Union>x\<in>multigraph_spec.delta_minus
+           (level_graph (dfs.Graph.digraph_abs E_simple) {s} -
+            {(u, v) |u v. distance (dfs.Graph.digraph_abs E_simple) s u = \<infinity>})
+           prod.snd x.
+         {xa. \<exists>uu. Some uu = realising_edges_lookup realising_edges x \<and> xa \<in> set uu})"
+        using realising_edges_result(1) realising_edges_result(3) helper_minus
+        by(auto intro: sum.mono_neutral_cong_right[OF _ _ _ refl]
+            simp add: multigraph_spec.delta_minus_def residual_level_graph_def
+            multigraph_spec.multi_level_graph_def Collect_bex_eq[symmetric]
+            multigraph_spec.multigraph_distance_set_def to_vertex_pair_fst_snd
+            level_graph_def E_simple_props(4) pos_es_props(1)  distance_set_def 
+            finite_\<EE> multigraph_spec.delta_minus_def[of "residual_level_graph \<f> s" sndv x]
+            residual_level_graph_in_E[of \<f> s] rev_finite_subset[of \<EE> "residual_level_graph \<f> s"])
+      have finite_if_list: "finite {x. \<exists>uu. Some uu = realising_edges_lookup realising_edges e \<and> x \<in> set uu}" for e
+        by(cases "realising_edges_lookup realising_edges e") auto
+      have same_big_sum_plus:
+        "sum (abstract_real_map (residual_flow_lookup rf))
+     (multigraph_spec.delta_plus (residual_level_graph \<f> s) fstv x) =
+     sum (abstract_real_map (residual_flow_lookup rf))
+     (\<Union>x\<in>multigraph_spec.delta_plus
+           (level_graph (dfs.Graph.digraph_abs E_simple) {s} -
+            {uu. \<exists>u. (\<exists>v. uu = (u, v)) \<and> distance (dfs.Graph.digraph_abs E_simple) s u = \<infinity>})
+           prod.fst x.
+         {xa. \<exists>uu. Some uu = realising_edges_lookup realising_edges x \<and> xa \<in> set uu})"
+        using realising_edges_result(1) realising_edges_result(3) helper_plus
+        by(auto intro: sum.mono_neutral_cong_right[OF _ _ _ refl]
+            simp add: multigraph_spec.delta_plus_def residual_level_graph_def
+            multigraph_spec.multi_level_graph_def Collect_bex_eq[symmetric]
+            multigraph_spec.multigraph_distance_set_def to_vertex_pair_fst_snd
+            level_graph_def E_simple_props(4) pos_es_props(1)  distance_set_def 
+            finite_\<EE> multigraph_spec.delta_minus_def[of "residual_level_graph \<f> s" sndv x]
+            residual_level_graph_in_E[of \<f> s] rev_finite_subset[of \<EE> "residual_level_graph \<f> s"])     
+      show ?thesis
+        using flow_network_axioms_for_simple_graph[OF blocking_flow_simple_correct(4), OF asm']
+          multigraph.delta_minus_finite[of prod.fst prod.snd id Pair 
+            "level_graph (dfs.Graph.digraph_abs E_simple) {s} - _"] 
+          multigraph.delta_plus_finite[of prod.fst prod.snd id Pair 
+            "level_graph (dfs.Graph.digraph_abs E_simple) {s} - _"] 
+          finite_if_list same_big_sum_minus same_big_sum_plus
+        by (auto simp add: find_blocking_flow_properties(5)[OF asm, simplified asm', simplified]
+            disjoint_multiple_sum[OF _ distinct_pairs_no_reaising_in_common] 
+            flow_network_def flow_network_spec.ex_def)
+    qed
+    have level_graph_simple_subset:
+      "level_graph (dfs.Graph.digraph_abs E_simple) {s} -
+              {uu.
+               \<exists>u. (\<exists>v. uu = (u, v)) \<and> distance (dfs.Graph.digraph_abs E_simple) s u = \<infinity>} 
+           \<subseteq> to_vertex_pair ` residual_level_graph \<f> s"
+      by(auto simp add: level_graph_def distance_set_def E_simple_props(4) pos_es_props(1)
+          residual_level_graph_def multigraph_spec.multi_level_graph_def
+          multigraph_spec.multigraph_distance_set_def to_vertex_pair_fst_snd)
+    show ?thesis
+    proof(rule flow_network_spec.is_s_t_flowI, goal_cases)
+      case 1
+      then show ?case 
+        using uflow by simp
+    next
+      case 2
+      then show ?case 
+        using same_excess blocking_flow_simple_correct(3)[OF asm']
+        by(auto elim!: flow_network_spec.is_s_t_flowE 
+            simp add: flow_network_spec.is_blocking_flow_def)
+    next
+      case 3
+      then show ?case
+        using  dVs_subset[OF level_graph_simple_subset]  blocking_flow_simple_correct(3)[OF asm']
+        by(auto elim!: flow_network_spec.is_s_t_flowE 
+            simp add: flow_network_spec.is_blocking_flow_def)
+    next
+      case 4
+      then show ?case 
+        using  dVs_subset[OF level_graph_simple_subset]  blocking_flow_simple_correct(3)[OF asm']
+        by(auto elim!: flow_network_spec.is_s_t_flowE 
+            simp add: flow_network_spec.is_blocking_flow_def)
+    next
+      case 5
+      then show ?case 
+        using   blocking_flow_simple_correct(3)[OF asm']
+        by(auto elim!: flow_network_spec.is_s_t_flowE 
+            simp add: flow_network_spec.is_blocking_flow_def)
+    next
+      case (6 x)
+      then show ?case 
+      proof(cases "x \<in> dVs (level_graph (dfs.Graph.digraph_abs E_simple) {s} -
+                  {uu. \<exists>u. (\<exists>v. uu = (u, v)) \<and>
+                       distance (dfs.Graph.digraph_abs E_simple) s u = \<infinity>})")
+        case True
+        then show ?thesis 
+          using same_excess  6  blocking_flow_simple_correct(3)[OF asm']         
+          by(auto elim!: flow_network_spec.is_s_t_flowE 
+              simp add: flow_network_spec.is_blocking_flow_def)
+      next
+        case False
+        have deltas_0:"e \<in> multigraph_spec.delta_minus (residual_level_graph \<f> s) sndv x \<Longrightarrow>
+                   abstract_real_map (residual_flow_lookup rf) e = 0" 
+          "e \<in> multigraph_spec.delta_plus (residual_level_graph \<f> s) fstv x \<Longrightarrow>
+                   abstract_real_map (residual_flow_lookup rf) e = 0" for e
+          using set_mp[OF dom_goal, of e] False
+          by(auto intro!: abstract_real_map_none 
+              simp add: multigraph_spec.delta_minus_def multigraph_spec.multigraph_distance_def 
+              E_simple_props(4) pos_es_props(1) residual_level_graph_def multigraph_spec.multi_level_graph_def
+              level_graph_def multigraph_spec.multigraph_distance_set_def distance_set_def
+              dom_def to_vertex_pair_fst_snd multigraph_spec.delta_plus_def)
+        then show ?thesis
+          by(auto simp add: flow_network_spec.ex_def comm_monoid_add_class.sum.neutral)
+      qed
+    qed
+  qed
+  show "residual_level_blocking_flow \<f> s t (abstract_real_map (residual_flow_lookup rf))"
+  proof(unfold residual_level_blocking_flow_def
+      flow_network_spec.is_blocking_flow_def multigraph_spec.multigraph_path_def,
+      rule ccontr, goal_cases)
+    case 1
+    then obtain p where p_prop:
+      "awalk UNIV (fstv (hd p)) (map to_vertex_pair p) (sndv (last p))"
+      "p \<noteq> []" "fstv (hd p) = s" "sndv (last p) = t" "set p \<subseteq> residual_level_graph \<f> s"
+      "\<And> e. e\<in>set p \<Longrightarrow> abstract_real_map (residual_flow_lookup rf) e < \<uu>\<^bsub>\<f>\<^esub>e"
+      using valid_s_t_flow by auto
+    have "set (map to_vertex_pair p) \<subseteq> (level_graph (dfs.Graph.digraph_abs E_simple) {s} -
+            {(u, v) |u v. distance (dfs.Graph.digraph_abs E_simple) s u = \<infinity>})"
+    proof(rule, goal_cases)
+      case (1 e)
+      then obtain ee where ee: "ee \<in> set p" "to_vertex_pair ee = e" by auto
+      then obtain p1 p2 where p1p2:"map to_vertex_pair p = p1@[e]@p2"
+        using "1" single_in_append split_list_last by force
+      have "distance (to_vertex_pair ` {uu \<in> \<EE>. 0 < \<uu>\<^bsub>\<f>\<^esub>uu}) s (prod.fst e) < \<infinity>"
+      proof(cases p1)
+        case Nil
+        hence "s = prod.fst e"
+          using p1p2 diff_is_res_circ p_prop(3) vs_to_vertex_pair_pres(1)
+          by auto
+        then show ?thesis 
+          using ee p_prop(5)
+          by(intro ord_class.ord_eq_less_trans[OF distance_0I, of _ _ _ \<infinity>])
+            (auto intro!: dVsI'(1) 
+              simp add: residual_level_graph_def multigraph_spec.multi_level_graph_def)
+      next
+        case (Cons a list)
+        have awalk_help: "awalk UNIV s p1 (prod.fst e)"
+          using awalk_fst_last p1p2 p_prop(1,3) by force
+        hence vwalk_found: "vwalk_bet (to_vertex_pair ` {uu \<in> \<EE>. 0 < \<uu>\<^bsub>\<f>\<^esub>uu}) s 
+                            (awalk_verts s p1) (prod.fst e)"
+          using Cons 
+          by(auto intro!: awalk_imp_vwalk  subset_mono_awalk'[of  UNIV]
+              set_mp[OF image_mono[OF  order.trans[OF p_prop(5)
+                    residual_level_graph_in_E_pos]], of _ to_vertex_pair, simplified]
+              simp add: cong[OF refl p1p2, of set, simplified] )
+        then show ?thesis 
+          by(auto intro!: order.strict_trans1[of _  _ \<infinity>, OF vwalk_bet_dist, simplified])
+      qed
+      then show ?case 
+        using set_mp[OF p_prop(5) ee(1)] 1 ee
+        by(auto simp add: level_graph_def E_simple_props(4) pos_es_props(1) distance_set_def
+            residual_level_graph_def multigraph_spec.multi_level_graph_def
+            multigraph_spec.multigraph_distance_set_def image_iff
+            split_pairs vs_to_vertex_pair_pres(1,2))
+    qed
+    moreover have pos_cap_old: "e\<in>set (map to_vertex_pair p) \<Longrightarrow>
+         ereal (abstract_real_map (lookup rfs) e) < ereal (u_simple e)" for e
+    proof(goal_cases)
+      case 1
+      then obtain ee where ee: "ee \<in> set p" "to_vertex_pair ee = e" by auto
+      obtain ds where ds: "realising_edges_lookup realising_edges e = Some ds"
+        "{ea |ea. ea \<in> set pos_es \<and> to_vertex_pair ea = e} \<noteq> {}"
+        using realising_edges_result(3)[of e]  pos_es_props(1)
+          set_mp[OF image_mono[OF order.trans[OF p_prop(5) residual_level_graph_in_E_pos]]
+            1[simplified]]
+        by auto
+      have ee_unsaturated: "abstract_real_map (residual_flow_lookup rf) ee < real_of_ereal \<uu>\<^bsub>\<f>\<^esub>ee"
+        using ee(1)   p_prop(5) residual_level_graph_in_E[of \<f> s]
+        by(unfold less_ereal.simps(1)[symmetric], subst ereal_real'[simplified in_mono not_infty_ereal])
+          (auto intro!: p_prop(6) intro: finite_rescapsE[of ee \<f>] )
+      have capacity_respected: "d \<in> \<EE> \<Longrightarrow> 0 < \<uu>\<^bsub>\<f>\<^esub>d \<Longrightarrow> 
+            abstract_real_map (residual_flow_lookup rf) d \<le> real_of_ereal (\<uu>\<^bsub>\<f>\<^esub>d)" for d
+        by(unfold ereal_less_eq(3)[symmetric], 
+            subst ereal_real'[simplified in_mono not_infty_ereal],
+            all \<open>cases "residual_flow_lookup rf d"\<close>)
+          (auto intro!: find_blocking_flow_properties(3)[OF asm]
+            elim: finite_rescapsE
+            simp add: abstract_real_map_none zero_ereal_def real_of_ereal_pos )
+      have finites: "finite {ea |ea. ea \<in> set pos_es \<and> to_vertex_pair ea = e}" by simp
+      show ?case 
+        using ee p_prop(5) residual_level_graph_in_E_pos  ee_unsaturated finites
+        by(auto intro!: ordered_cancel_comm_monoid_add_class.sum_strict_mono_strong[of _ ee] 
+            capacity_respected 
+            simp add: pos_es_props(1) find_blocking_flow_properties(5)[OF asm,
+              simplified asm' option.sel]
+            u_simple_is ds realising_edges_result(1)[OF ds(1)])
+    qed
+    moreover have "multigraph_spec.multigraph_path prod.fst prod.snd id (map to_vertex_pair p)"
+      using awalk_fst_last  p_prop(1)
+      by(force simp add: multigraph_spec.multigraph_path_def) 
+    moreover have "prod.fst (hd (map to_vertex_pair p)) = s"
+      using awalk_hd[OF p_prop(1)] p_prop(2,3)
+      by(cases p) auto
+    moreover have "prod.snd (last (map to_vertex_pair p)) = t"
+      using awalk_last[OF p_prop(1)] p_prop(2,4)
+      by(cases p) auto
+    ultimately show False
+      using  blocking_flow_simple_correct(3)[OF asm'] p_prop(2)
+      by(unfold flow_network_spec.is_blocking_flow_def) blast
+  qed
 qed
 
 
 end
+
 end
