Dinic/Multigraph_Collapse_and_Split.thy
@@ -1,0 +1,473 @@
+theory Multigraph_Collapse_and_Split
+  imports (*Directed_Set_Graphs.Multigraph*) "HOL-Eisbach.Eisbach"
+          Flow_Theory.Blocking_Flow
+begin
+
+locale split_weight_single_spec = 
+  fixes   add::"'w \<Rightarrow> 'w \<Rightarrow> 'w" ("_ w+ _")
+  and   subtr::"'w \<Rightarrow> 'w \<Rightarrow> 'w" ("_ w- _")
+  and   zero::"'w" ("w0")
+  and    wleq::"'w \<Rightarrow> 'w \<Rightarrow> bool" ("_ w\<le> _")
+  and   wless::"'w \<Rightarrow> 'w \<Rightarrow> bool" ("_ w< _")
+  and   weq::"'w \<Rightarrow> 'w \<Rightarrow> bool"   ("_ w= _")
+ (* and   iterate::"('x \<Rightarrow> ('map \<times> 'w) \<Rightarrow> ('map \<times> 'w))
+           \<Rightarrow> 'x_set \<Rightarrow>  ('map \<times> 'w) \<Rightarrow> 'map"*)
+  and update::"'map \<Rightarrow> 'x \<Rightarrow> 'w \<Rightarrow> 'map"
+  and lookup::"'map \<Rightarrow> 'x \<Rightarrow> 'w option"
+  and map_empty::'map
+begin
+
+fun split where 
+"split u [] W mp= mp"|
+"split u (x#xs) W mp= 
+   (if W w= w0 then mp
+    else if W w\<le> u x then update mp x W
+    else split u xs (W w-  u x) (update mp x (W w- (W w- u x))))"
+
+end
+
+locale split_weight_single =
+  split_weight_single_spec where
+add = "add::'w \<Rightarrow> 'w \<Rightarrow> 'w"  for add ("_ w+ _")
++ assumes  w_add_assoc:"\<And>a b c. ((a w+ b) w+ c) = (a w+ (b w+ c))"
+and     w_add_comm: "\<And>a b. (a w+ b) = (b w+ a)"
+and     w0_let_ntr: "\<And>a. (w0 w+ a) = a"
+and     less_def:   "\<And>x y::'w. (x w< y) = (x w\<le> y \<and> \<not> y w\<le> x)"
+and     less_refl: "\<And>x::'w. x w\<le> x" 
+and     less_trans: "\<And>x y z::'w. x w\<le> y \<Longrightarrow> y w\<le> z \<Longrightarrow> x w\<le> z"
+        (*"\<And>x y. x \<le> y \<Longrightarrow> y \<le> x \<Longrightarrow> x = y"
+        "\<And>a b::'w. (a \<le> b) = (\<exists>c. b = a w+ c)"
+        "\<And>a b::'w. a \<le> b \<Longrightarrow> b w- a w+ a = b"
+        "\<And>a b c. a - b - c = a - (b + c)"*)
+begin
+
+lemma split_lemma:
+  assumes "foldr add (map u xs) w0 w= W"
+  shows   "(foldr (\<lambda> x w. (the (lookup (split u xs W map_empty) x)) w+ w) xs w0)
+                w= W"
+          "\<And> x. x \<in> set xs
+            \<Longrightarrow> (the (lookup (split u xs W map_empty) x)) w\<le> u x"
+  sorry
+
+
+
+
+
+  oops
+
+split_weight_spec +
+assumes w_add_assoc:"\<And>a b c. ((a w+ b) w+ c) = (a w+ (b w+ c))"
+and     w_add_comm: "\<And>a b. a w+ b = b w+ a"
+and     w0_let_ntr: "\<And>a. w0 w+ a = a"
+and     less_def:   "\<And>x y::'w. (x < y) = (x \<le> y \<and> \<not> y \<le> x)"
+and     less_refl: "\<And>x::'w. x \<le> x" 
+and     less_trans: "\<And>x y z::'w. x \<le> y \<Longrightarrow> y \<le> z \<Longrightarrow> x \<le> z"
+        (*"\<And>x y. x \<le> y \<Longrightarrow> y \<le> x \<Longrightarrow> x = y"
+        "\<And>a b::'w. (a \<le> b) = (\<exists>c. b = a w+ c)"
+        "\<And>a b::'w. a \<le> b \<Longrightarrow> b w- a w+ a = b"
+        "\<And>a b c. a - b - c = a - (b + c)"*)
+
+
+
+
+
+
+
+
+  oops
+
+
+
+
+
+
+fun find_f where
+"find_f g acc [] f = f"|
+"find_f g acc [e] f= (\<lambda> d. if d = e then acc else f d)"|
+"find_f g acc (e#es) f= (if acc \<le> g e then (\<lambda> d. if d = e then acc else f d)
+                        else find_f g (acc - g e) es (\<lambda> d. if d = e then acc - (acc -  g e) else f d))"
+
+lemma e_not_in_no_change:"e \<notin> set es \<Longrightarrow> find_f g acc es f e = f e"
+  by(induction g acc es f arbitrary: e rule: find_f.induct )
+     auto
+
+lemma find_f_init_cong:
+  assumes "\<And> e. e \<in> set es \<Longrightarrow> f e = f' e"
+  shows  "e \<in> set es \<Longrightarrow> find_f g acc es f e = find_f g acc es f' e"
+  using assms
+proof(induction g acc es f arbitrary: f' e rule: find_f.induct )
+  case (1 g acc f)
+  then show ?case by simp
+  next
+  case (2 g acc e f)
+  then show ?case by simp
+next
+  case (3 g acc d v va f )
+  show ?case 
+    apply (subst find_f.simps(3))+
+    apply(cases "acc \<le> g d")
+    subgoal
+      apply(subst if_P[of "acc \<le> g d"])
+       apply simp
+      apply(subst if_P[of "acc \<le> g d"])
+       apply simp
+      using 3(2,3) by auto
+    subgoal
+      apply(subst if_not_P[of "acc \<le> g d"])
+       apply simp
+      apply(subst if_not_P[of "acc \<le> g d"])
+       apply simp
+      apply(cases "e \<in> set (v #va)")
+      subgoal
+      apply(rule 3(1))
+          apply simp
+         apply simp
+        apply simp
+        using 3(2,3) by simp
+      subgoal
+        apply(subst e_not_in_no_change)
+         apply simp
+        apply(subst e_not_in_no_change)
+         apply simp
+        using 3(2,3) by simp
+      done
+    done
+qed
+  
+  
+lemma 
+  assumes "A \<subseteq> \<Union> (g ` (set es))" "es \<noteq> []" "distinct es"
+  shows       "\<exists> f. (\<forall> e \<in> set es. f e \<subseteq> g e) \<and> \<Union> (f ` (set es)) = A"
+proof-
+  define f where "f = find_f g A es (\<lambda> e. {})"
+  have prop1:"\<Union> (f ` set es) = A"
+    using assms(1,2,3)
+    unfolding f_def
+  proof(induction es arbitrary: A)
+    case Nil
+    then show ?case by simp
+  next
+    case (Cons e es)
+    note IH = this
+    show ?case 
+    proof(cases es)
+      case Nil
+      show ?thesis 
+        apply(subst Nil, subst find_f.simps, subst Nil)
+        by simp
+    next
+      case (Cons d list)
+      show ?thesis 
+        apply(subst Cons)
+        apply(subst find_f.simps)
+        apply(cases "A \<subseteq> g e")
+        subgoal
+          apply(subst if_P[of "A \<subseteq> g e"])
+           apply simp
+          apply(subst set_simps(2))
+          apply(subst Union_image_insert)
+          using IH(4) by simp
+        subgoal
+          apply(subst if_not_P[of "A \<subseteq> g e"])
+           apply simp
+          apply(subst set_simps(2))
+          apply(subst Union_image_insert)
+          apply(subst e_not_in_no_change[of e "d#list" g "A - g e"])
+          using IH(4) Cons apply simp
+          apply(subst if_P[of "e = e"])
+           apply simp
+          unfolding Cons[symmetric]
+         apply(subst image_cong[OF refl  find_f_init_cong[of
+               es "(\<lambda>d. if d = e then A - (A - g e) else {})" "\<lambda> x.  {}" _ g "A - g e"], of "set es" "\<lambda> x. x"]
+        )
+          apply(subst if_not_P)
+          using IH(4) Cons apply force
+            apply simp        
+          apply simp
+          apply(subst IH(1)) (*interesting*)
+          using IH(2) apply force
+          using Cons apply simp
+          using IH(4) apply simp (*interesting*)
+          by auto
+        done
+    qed
+  qed
+  have prop2:"e\<in>set es \<Longrightarrow> f e \<subseteq> g e" for e
+    unfolding f_def
+    using assms(1,2,3)
+  proof(induction es arbitrary: A)
+    case Nil
+    then show ?case by simp
+  next
+    case (Cons d es)
+    note IH = this
+    show ?case 
+    proof(cases es)
+      case Nil
+      then show ?thesis 
+        using IH(2,3) 
+        unfolding Nil
+        apply(subst find_f.simps)
+        by simp
+    next
+      case (Cons a list)
+      show ?thesis 
+        unfolding Cons
+        apply(subst find_f.simps)
+        apply(cases "A \<subseteq> g d")
+        subgoal
+          apply(subst if_P[of "A \<subseteq> g d"])
+           apply simp
+          by auto
+        subgoal
+          apply(subst if_not_P[of "A \<subseteq> g d"])
+           apply simp
+          apply(cases "d = e")
+          subgoal
+            apply(subst e_not_in_no_change)
+            using IH(5) Cons apply simp
+            apply(subst if_P)
+             apply simp (*interesting*)
+            by auto
+          subgoal
+            unfolding Cons[symmetric]
+            apply(subst find_f_init_cong[of
+               es "(\<lambda>da. if da = d then A - (A - g d) else {})" "\<lambda> x.  {}" _ g "A - g d"])
+            apply(subst if_not_P)
+            using IH(5) Cons apply auto[1]
+            apply simp
+            using IH(2) Cons apply simp
+            apply(rule IH(1))
+            using IH(2) Cons apply simp (*interesting*)
+            using IH(3) apply force
+            using Cons apply simp
+            using IH(5) apply simp
+            done
+          done
+        done
+    qed
+  qed
+  show ?thesis
+    apply(rule exI[of _ f])
+    using prop1 prop2 by simp
+ (* have "(\<And> e. e\<in>set es \<Longrightarrow> f' e \<subseteq> g e) \<Longrightarrow> \<Union> (f' ` set es) = A 
+           \<Longrightarrow> (\<And> e. e \<in> set es \<Longrightarrow> f' e \<subseteq> f e) \<Longrightarrow> \<exists> e \<in> set es. f' e \<subset> f e \<Longrightarrow> False" for f'
+   *)
+qed
+
+
+
+typ "'a set"
+
+typ nat
+
+context canonically_ordered_monoid_add begin end
+context ordered_cancel_comm_monoid_diff  begin end
+
+context comm_monoid_diff begin
+end             
+context cancel_comm_monoid_add begin
+end
+context comm_monoid_add begin end
+context cancel_ab_semigroup_add begin end (* problem*)
+context ordered_ab_semigroup_add_imp_le begin end
+context ordered_cancel_ab_semigroup_add begin end
+context ordered_ab_semigroup_add begin end
+
+
+class comm_monoid_monus = 
+  canonically_ordered_monoid_add + 
+   minus +
+  assumes add_diff_cancel_left' [simp]: "a  \<le> b \<Longrightarrow> (b -a) + a = b"
+  assumes diff_diff_add [algebra_simps, algebra_split_simps,
+                         field_simps, field_split_simps]:
+                            "a - b - c = a - (b + c)"
+  assumes diff_leq_minuend: "a - b \<le> a"
+  assumes zero_diff [simp]: "0 - a = 0"
+begin
+
+lemma "a - (a - b) \<le> b" 
+  unfolding le_iff_add
+  find_theorems "(_::'a) - _"
+  find_theorems "_ \<le> (_::'a)"
+
+(*
+lemma 
+  assumes "c +b = a" "(\<And> d. d + b = a \<Longrightarrow> c \<le> d)" 
+  shows"c = a -b"
+proof-
+  have "c \<le> a - b" 
+    using add_commute assms(1,2) local.add_diff_cancel_left' local.le_iff_add
+    by blast
+  moreover have "c \<ge> a - b"
+    sledgehammer
+ 
+  find_theorems "(_::'a) \<le> _"
+*)
+end
+
+instantiation set:: (type) comm_monoid_monus 
+begin
+
+definition "plus_set = Set.union"
+definition "zero_set = {}"
+
+instance proof
+  show "\<And>(a::'a set) b c. a + b + c = a + (b + c)"
+       "\<And>(a::'a set) b. a + b = b + a"
+       "\<And>(a::'a set). 0 + a = a"
+       "\<And>a b. (a \<subseteq> b) = (\<exists>c. b = a + c)"
+       "\<And>a b. a \<subseteq> b \<Longrightarrow> b - a + a = b"
+       "\<And>(a::'a set) b c. a - b - c = a - (b + c)"
+       "\<And>(a::'a set). 0 - a = 0"
+       "\<And>(a::'a set) b. a - b \<subseteq> a"
+    by(auto simp add: plus_set_def zero_set_def)
+qed
+end
+
+instantiation nat:: comm_monoid_monus 
+begin
+
+instance proof
+  show "\<And>(a::nat) b. a \<le> b \<Longrightarrow> b - a + a = b"
+       "\<And>(a::nat) b c. a - b - c = a - (b + c)"
+       "\<And>(a::nat). 0 - a = 0"
+       "\<And>a b::nat. a - b \<le> a"
+    by(auto simp add: plus_set_def zero_set_def)
+qed
+end
+(*
+definition pos_real_rel::"real \<Rightarrow> real \<Rightarrow> bool" where
+"pos_real_rel x y = ( \<bar> x \<bar> = \<bar> y \<bar>)"
+
+quotient_type pos_real = real / pos_real_rel
+ morphisms Rep_Integ Abs_Integ
+ by(auto intro!: equivpI reflpI sympI transpI simp add: pos_real_rel_def)
+
+find_theorems "_::pos_real"
+typ real
+term Abs_pos_real
+term Rep_pos_real
+*)
+(*
+datatype real_wrapper = wrap real 
+
+fun the_real where "the_real (wrap x) = x"
+
+instantiation real_wrapper::  comm_monoid_monus 
+begin
+
+definition "zero_real_wrapper = wrap 0"
+
+definition "minus_real_wrapper (x::real_wrapper) (y::real_wrapper) =
+            wrap ( max (0::real) (the_real x  - the_real y))"
+
+definition "less_eq_real_wrapper (x::real_wrapper) (y::real_wrapper) =
+           (the_real x  \<le>  the_real y )"
+
+definition "less_real_wrapper (x::real_wrapper) (y::real_wrapper) =
+           ( the_real x  < the_real y)"
+
+definition "plus_real_wrapper (x::real_wrapper) (y::real_wrapper) =
+            wrap ( max (0::real) (the_real x  + the_real y ))"
+
+instance proof
+  show "\<And>(a::real_wrapper) b c. a + b + c = a + (b + c)"
+       "\<And>(a::real_wrapper) b. a + b = b + a"
+       "\<And>(a::real_wrapper). 0 + a = a"
+    apply(auto simp add: plus_real_wrapper_def zero_real_wrapper_def)
+   *)
+
+datatype ereal_wrapper = wrap ereal
+
+fun the_ereal where
+"the_ereal (wrap x) = x"
+text \<open>An interpretation of ereal wrappers as commutative monoid with monus.
+This is suitable for shortest paths.\<close>
+instantiation ereal_wrapper:: comm_monoid_monus 
+begin
+
+definition "plus_ereal_wrapper (x::ereal_wrapper) y
+           = wrap (min (the_ereal x) (the_ereal y))"
+definition "zero_ereal_wrapper = wrap PInfty"
+definition "minus_ereal_wrapper (x::ereal_wrapper) y =
+           (if the_ereal x < the_ereal y then x else wrap PInfty)"
+definition "less_eq_ereal_wrapper (x::ereal_wrapper) y =
+             (the_ereal x \<ge> the_ereal y)"
+definition "less_ereal_wrapper (x::ereal_wrapper) y =
+             (the_ereal x > the_ereal y)"
+
+instance proof
+  show "(a \<le> b) = (\<exists>c. b = a + c)" for a b::ereal_wrapper
+    by(auto simp add:  plus_ereal_wrapper_def 
+                       less_eq_ereal_wrapper_def less_ereal_wrapper_def
+              intro: the_ereal.elims intro!: exI[of _ b])
+  show "a \<le> b \<Longrightarrow> b - a + a = b" for a b::ereal_wrapper
+    by(cases a, all \<open>cases b\<close>)
+      (auto simp add: plus_ereal_wrapper_def minus_ereal_wrapper_def
+                         less_ereal_wrapper_def less_eq_ereal_wrapper_def)
+ show " 0 + a = a" for a::ereal_wrapper
+    by(cases a)
+      (auto simp add: plus_ereal_wrapper_def zero_ereal_wrapper_def)
+  show 
+"\<And>(a::ereal_wrapper) b c. a + b + c = a + (b + c)"
+"\<And>(a::ereal_wrapper) b. a + b = b + a"
+"\<And>a::ereal_wrapper. 0 - a = 0"
+"\<And>(x::ereal_wrapper) y. (x < y) = (x \<le> y \<and> \<not> y \<le> x)"
+"\<And>x::ereal_wrapper. x \<le> x"
+"\<And>(x::ereal_wrapper) y z. x \<le> y \<Longrightarrow> y \<le> z \<Longrightarrow> x \<le> z"
+"\<And>(x::ereal_wrapper) y. x \<le> y \<Longrightarrow> y \<le> x \<Longrightarrow> x = y"
+"\<And>(a::ereal_wrapper) b c. a - b - c = a - (b + c)"
+"\<And>a b::ereal_wrapper. a - b \<le> a"
+    using  min.commute 
+    by(auto simp add: zero_ereal_wrapper_def minus_ereal_wrapper_def
+                      plus_ereal_wrapper_def min.assoc 
+                      less_eq_ereal_wrapper_def less_ereal_wrapper_def
+               intro: the_ereal.elims )
+qed
+end
+
+typedef pos_real = "{x::real | x. x \<ge> 0}"
+  morphisms real_of_pos_real pos_real
+  by auto
+print_theorems
+
+find_theorems "_::pos_real"
+
+code_datatype pos_real 
+setup_lifting type_definition_pos_real
+
+
+lift_definition plus::"pos_real \<Rightarrow> pos_real \<Rightarrow> pos_real" 
+    is "\<lambda> x y. ( x +  y)"
+  by simp
+
+lift_definition one::"pos_real" 
+    is "1"
+  by simp
+
+lift_definition zero::"pos_real" 
+    is "0"
+  by simp
+
+lemmas [code abstype] = pos_real.real_of_pos_real_inverse
+real_of_pos_real_inject plus_def one_def zero_def
+
+declare [[coercion_enabled]]
+
+instantiation pos_real::numeral
+begin
+
+
+definition "plus_pos_real (x::pos_real) y
+  = plus x y"
+
+instance proof
+  show "\<And> (a::pos_real) b c. a + b + c = a + (b + c)"
+    apply(auto simp add: plus_pos_real_def) 
+    sorry
+qed
+end
+
+value "(1::pos_real)"
+lemma "(1::pos_real) = undefined" 
